\documentclass{masterthesis}

\usepackage{hyperref} % links
\usepackage{graphicx}
\usepackage{amsmath}
\usepackage{amssymb}
\usepackage{qcircuit}
\usepackage{braket}
\usepackage{float}
\usepackage[toc,page]{appendix}

\begin{document}

\title{Exercises 8.23 and 9.21 - Nielsen and Chuang}

\author{Lorenzo La Corte}

\advisor{}

\examiner{}

\maketitle

\section*{8.23, Amplitude Damping of a Dual-Rail Qubit}

A dual-rail qubit is defined as
\begin{equation}
    \ket{\psi}=a\ket{01}+b\ket{10}
\end{equation}

Applying $\varepsilon_{A D} \otimes \varepsilon_{A D}$ to $\rho=\ket{\psi}\bra{\psi}$ produces a new state $\rho'$, according to the following operator sum representation:
\begin{equation}
    (\varepsilon_{A D} \otimes \varepsilon_{A D})(\rho) = \sum_{i} E_{i} \rho E_{i}^{\dagger} = \rho'
\end{equation}

Where the Kraus operators $E_{i}$ are given by the tensor product of the Kraus operators $E_{j}^{s}$, which are the operation elements of the Amplitude Damping acting on a single qubit:
\begin{equation}
    E_{0}^{s} = \begin{pmatrix} 1 & 0 \\ 0 & \sqrt{1-\gamma} \end{pmatrix}, \quad E_{1}^{s} = \begin{pmatrix} 0 & \sqrt{\gamma} \\ 0 & 0 \end{pmatrix}
\end{equation}

Thus, the Kraus operators $E_{i}$ the Amplitude Damping acting on two qubits are given by:
\begin{equation}
    E_{00} = E_{0}^{s} \otimes E_{0}^{s}, \quad , \quad E_{01} = E_{0}^{s} \otimes E_{1}^{s}, \quad E_{10} = E_{1}^{s} \otimes E_{0}^{s}, \quad E_{11} = E_{1}^{s} \otimes E_{1}^{s}
\end{equation}

\begin{multline}\label{eq:op-el-1}
    E_{00} = \ket{00}\bra{00} + \sqrt{1-\gamma}\ket{01}\bra{01} + \sqrt{1-\gamma}\ket{10}\bra{10} + (1-\gamma)\ket{11}\bra{11} = \\
    = \begin{pmatrix} 1 & 0 & 0 & 0 \\ 0 & \sqrt{1-\gamma} & 0 & 0 \\ 0 & 0 & \sqrt{1-\gamma} & 0 \\ 0 & 0 & 0 & 1-\gamma \end{pmatrix}
\end{multline}
\begin{equation}\label{eq:op-el-2}
    E_{01} = \sqrt{\gamma}\ket{00}\bra{01} + \sqrt{\gamma}\sqrt{1-\gamma}\ket{10}\bra{11}
    = \begin{pmatrix} 0 & \sqrt{\gamma} & 0 & 0 \\ 0 & 0 & 0 & 0 \\ 0 & 0 & 0 & \sqrt{\gamma}\sqrt{1-\gamma} \\ 0 & 0 & 0 & 0 \end{pmatrix}
\end{equation}
\begin{equation}\label{eq:op-el-3}
    E_{10} = \sqrt{\gamma}\ket{00}\bra{01} + \sqrt{\gamma}\sqrt{1-\gamma}\ket{01}\bra{11}  
    = \begin{pmatrix} 0 & 0 & \sqrt{\gamma} & 0 \\ 0 & 0 & 0 & \sqrt{\gamma}\sqrt{1-\gamma} \\ 0 & 0 & 0 & 0 \\ 0 & 0 & 0 & 0 \end{pmatrix}
\end{equation}
\begin{equation}\label{eq:op-el-4}
    E_{11} = \gamma \ket{00}\bra{11}
    = \begin{pmatrix} 0 & 0 & 0 & \gamma \\ 0 & 0 & 0 & 0 \\ 0 & 0 & 0 & 0 \\ 0 & 0 & 0 & 0 \end{pmatrix}
\end{equation}

% If we restrict the operator to the span {$\ket{01}$, $\ket{10}$}, we get the operators:
% \begin{equation}
%     E_{0}^{s} = \sqrt{1-\gamma} I
% \end{equation}
% \begin{equation}
%     E_{1}^{s} = \sqrt{\gamma}|00\rangle\langle 01| = \sqrt{\gamma}\begin{pmatrix} 0 & 1 & 0 & 0 \\ 0 & 0 & 0 & 0 \\ 0 & 0 & 0 & 0 \\ 0 & 0 & 0 & 0 \end{pmatrix}
% \end{equation}
% \begin{equation}
%     E_{2} = \sqrt{\gamma}|00\rangle\langle 10| = \sqrt{\gamma}\begin{pmatrix} 0 & 0 & 1 & 0 \\ 0 & 0 & 0 & 0 \\ 0 & 0 & 0 & 0 \\ 0 & 0 & 0 & 0 \end{pmatrix}
% \end{equation}

We have that
\begin{equation}
    E_{00} \rho E_{00}^{\dagger} = (1-\gamma) \rho
\end{equation}
\begin{equation}
    E_{01} \rho E_{01}^{\dagger} = |a|^2 \gamma \ket{00}\bra{00}
\end{equation}
\begin{equation}
    E_{10} \rho E_{10}^{\dagger} = |b|^2 \gamma \ket{00}\bra{00}
\end{equation}
\begin{equation}
    E_{11} \rho E_{11}^{\dagger} = 0
\end{equation}

And so, the application of these operators to the state $\rho$ produces the state $\rho'$, which is given by:
\begin{equation}\label{eq:ad-dual-rail}
    \rho' = (1-\gamma)\begin{pmatrix} 0 & 0 & 0 & 0 \\ 0 & |a|^{2} & a b^{*} & 0 \\ 0 & a^{*} b & |b|^{2} & 0 \\ 0 & 0 & 0 & 0 \end{pmatrix} + \gamma\begin{pmatrix} 1 & 0 & 0 & 0 \\ 0 & 0 & 0 & 0 \\ 0 & 0 & 0 & 0 \\ 0 & 0 & 0 & 0 \end{pmatrix}
\end{equation}

Thus, with probability $\gamma$, the state is projected to $\ket{00}$, orthogonal to $\ket{\psi}$, while with probability $1-\gamma$, the state is unchanged. 

% This means that the state $\ket{00}$ can be used to detect amplitude damping errors with measurement operators:
% \begin{equation}
%     M_{0} = \ket{00}\bra{00} \quad \text{projector on} \operatorname{span}\{\ket{00}\}
% \end{equation}
% \begin{equation}
%     M_{1} = \ket{01}\bra{01} + \ket{10}\bra{10} + \ket{11}\bra{11} \quad \text{projector on} \operatorname{span}\{\ket{01}, \ket{10}, \ket{11}\}
% \end{equation}

\paragraph*{Proof}
We can get the same result considering the effect of amplitude damping on the first qubit and second qubit separetely, respectively associated to the third and fourth qubit for the environment, which both start from the state 0.

Since the circuit of the amplitude damping on a single qubit is the following:
\begin{align}
    \Qcircuit @C=1em @R=1.2em {
        \lstick{\rho} & \qw & \ctrl{1} & \targ & \rstick{\rho'} \qw \\
        \lstick{\ket{0}} & \qw & \gate{R_y(\theta)} & \ctrl{-1} & \meter \qw
      }          
\end{align}

So the one for the amplitude damping on a dual-rail qubit is:
\begin{align}
    \Qcircuit @C=1em @R=1.2em {
        & \qw & \ctrl{2} & \targ & \qw & \qw & \qw \\
        & \qw & \qw & \qw & \ctrl{2} & \targ & \qw \\
        \lstick{\ket{0}} & \qw & \gate{R_y(\theta)} & \ctrl{-2} & \qw & \qw & \meter \qw \\
        \lstick{\ket{0}} & \qw & \qw & \qw & \gate{R_y(\theta)} & \ctrl{-2} & \meter \qw
      }          
\end{align}

Algebraically, we start from a tensor product state:
\begin{equation}
    \omega_0 = \ket{\psi}\ket{00} = a\ket{0100} + b\ket{1000}
\end{equation}

Applying, in sequence:
\begin{enumerate}
    \item a controlled rotation on the Y axis: $CR_{y}(\theta)_{1,3}$,
    \item a controlled not $CX_{3,1}$
\end{enumerate}

\begin{equation}
    \omega_1 = CX_{3,1} CR_{y}(\theta)_{1,3} (\omega_0)
\end{equation}

The rotation on the Y axis of $\theta$ is defined as:
\begin{equation}
    R_y(\theta) = \begin{pmatrix} \cos\frac{\theta}{2} & -\sin\frac{\theta}{2} \\ \sin\frac{\theta}{2} & \cos\frac{\theta}{2} \end{pmatrix}
\end{equation}

And acts on $\ket{0}$ as following:
\begin{equation}
    R_y(\theta)\ket{0} = \cos\frac{\theta}{2}\ket{0} + \sin\frac{\theta}{2}\ket{1}
\end{equation}

Only the second term of $\omega_0$ is rotated, as it is the only one with the first qubit set to 1, producing
\begin{equation}
    \omega_1 = CX_{3,1} (a\ket{0100} + b\cos\frac{\theta}{2}\ket{1000} + b\sin\frac{\theta}{2}\ket{1010})
\end{equation}

Then the CNOT flips only the third term, producing
\begin{equation}
    \omega_1 = a\ket{0100} + b\cos\frac{\theta}{2}\ket{1000} + b\sin\frac{\theta}{2}\ket{0010}
\end{equation}

This is the state of the system after having applied amplitude damping on the first qubit.

Then, the effect of the amplitude damping on the second qubit corresponds to the application, in sequence, of another pair of gates (controlled rotation and controlled not), on the second and fourth qubit:

\begin{equation}
    \omega_2 = CX_{4,2} CR_{y}(\theta)_{2,4} (\omega_1)
\end{equation}
\begin{equation}
    \omega_2 = CX_{4,2} (a\cos\frac{\theta}{2}\ket{0100} + a\sin\frac{\theta}{2}\ket{0101} + b\cos\frac{\theta}{2}\ket{1000} + b\sin\frac{\theta}{2}\ket{0010})
\end{equation}
\begin{equation}
    \omega_2 = a\cos\frac{\theta}{2}\ket{0100} + a\sin\frac{\theta}{2}\ket{0001} + b\cos\frac{\theta}{2}\ket{1000} + b\sin\frac{\theta}{2}\ket{0010}
\end{equation}

Let
\begin{equation}
    \ket{\phi} = \omega_2 = a\cos\frac{\theta}{2}\ket{0100} + a\sin\frac{\theta}{2}\ket{0001} + b\cos\frac{\theta}{2}\ket{1000} + b\sin\frac{\theta}{2}\ket{0010}
\end{equation}
our target is to trace out the environment from this state.

To do that, we pass to the density matrix representation $\ket{\phi}\bra{\phi}$, which has 16 terms, deriving from the tensor product of the 4 terms of $\ket{\phi}$ with their conjugates:
\begin{align}
    \ket{\phi}\bra{\phi} &= (a\cos\frac{\theta}{2}\ket{0100} + a\sin\frac{\theta}{2}\ket{0001} + b\cos\frac{\theta}{2}\ket{1000} + b\sin\frac{\theta}{2}\ket{0010}) \nonumber \\
    &(a^{*}\cos\frac{\theta}{2}\bra{0100} + a^{*}\sin\frac{\theta}{2}\bra{0001} + b^{*}\cos\frac{\theta}{2}\bra{1000} + b^{*}\sin\frac{\theta}{2}\bra{0010})
\end{align}

We can simplify calculations by taking the trace of the environment while multiplying the terms: we discard the terms that do not have matching qubits for the environment.

In particular, we have 4 terms coming from the multiplications of the terms by themselves (where obviously the environment bits are matching), plus 2 more coming from the multiplication of the first and the third terms of $\ket{\phi}$:

\begin{align}
    Tr_e(\ket{\phi}\bra{\phi}) &= |a|^2 \cos^2 \frac{\theta}{2}\ket{01}\bra{01} + |a|^2 \sin^2 \frac{\theta}{2}\ket{00}\bra{00} + |b|^2 \cos^2 \frac{\theta}{2}\ket{10}\bra{10} \\
    & + |b|^2 \sin^2 \frac{\theta}{2}\ket{00}\bra{00} + a b^{*} \cos^2 \frac{\theta}{2} \ket{01}\bra{10} + a^{*} b \cos^2 \frac{\theta}{2} \ket{10}\bra{01} 
\end{align}

Which can be simplified to 
\begin{align}
    Tr_e(\ket{\phi}\bra{\phi}) &= \sin^2 \frac{\theta}{2}\ket{00}\bra{00} \\ 
    & + |a|^2 \cos^2 \frac{\theta}{2}\ket{01}\bra{01} + a b^{*} \cos^2 \frac{\theta}{2} \ket{01}\bra{10} \\
    & + a^{*} b \cos^2 \frac{\theta}{2} \ket{10}\bra{01} + |b|^2 \cos^2 \frac{\theta}{2}\ket{10}\bra{10}
\end{align}

Let $\gamma=sin^2\frac{\theta}{2}$
\begin{align}
    Tr_e(\ket{\phi}\bra{\phi}) &= \gamma\ket{00}\bra{00} \\ 
    & + (1-\gamma) |a|^2 \ket{01}\bra{01} + (1-\gamma) a b^{*} \ket{01}\bra{10} \\
    & + (1-\gamma) a^{*} b \ket{10}\bra{01} + (1-\gamma) |b|^2 \ket{10}\bra{10} \\
    &= \rho'
\end{align}
thus, we got the same result as \hyperref[eq:ad-dual-rail]{Eq.13}, proving that the amplitude damping on 2 qubits is described by the operation elements \hyperref[eq:op-el-1]{$E_{00}$}, \hyperref[eq:op-el-2]{$E_{01}$}, \hyperref[eq:op-el-3]{$E_{10}$}, \hyperref[eq:op-el-4]{$E_{11}$}.

\newpage
\section*{9.21, Relationship between Fidelity and Trace Distance}

The relationship between fidelity and trace distance of two mixed states is defined as
\begin{equation}
    1 - F(\rho, \sigma) \leq D(\rho, \sigma)
\end{equation}

\paragraph*{Theorem}
When comparing pure states and mixed states it is possible to make a stronger statement
\begin{equation}
    1 - F(\ket{\psi}, \sigma)^2 \leq D(\ket{\psi}, \sigma)
\end{equation}
where $\ket{\psi}$ is a pure state and $\sigma$ is a mixed state.

\paragraph*{Proof}
Consider the definition of fidelity between a pure and a mixed state
\begin{equation}
    F(\ket{\psi}, \sigma) = \sqrt{\bra{\psi}\sigma\ket{\psi}}
\end{equation}

Let $E_m$ set of POVM, such that
\begin{equation}
    p_m = Tr(\ket{\psi}\bra{\psi} E_m) \quad \quad q_m = Tr(\sigma E_m)
\end{equation}
where $p_m$ and $q_m$ are the probability distributions of respectively $\ket{\psi}$ and $\sigma$.

We can rewrite $p_m$ as
\begin{equation}
    p_m = Tr(\ket{\psi}\bra{\psi} E_m) = \sum_{i} \bra{i} \ket{\psi}\bra{\psi} E_m \ket{i} = \bra{\psi}E_m\ket{\psi}
\end{equation}

And write the fidelity as
\begin{equation}
    F(\ket{\psi}, \rho) = \sum_{m} \sqrt{p_m q_m} 
\end{equation}

We can prove this statement by noticing that $\bra{\psi}E_m\ket{\psi} = 1$ if and only if $E_m = \ket{\psi}\bra{\psi}$, thus:
\begin{align}
    \sum_{m} \sqrt{p_m q_m} = \sum_{m} \sqrt{\bra{\psi}E_m\ket{\psi} Tr(\sigma E_m)} = \\
    = \sqrt{\bra{\psi}\ket{\psi}\bra{\psi}\ket{\psi} Tr(\sigma \ket{\psi}\bra{\psi})} = \\
    = \sqrt{\sum_{i} \bra{i} \sigma \ket{\psi}\bra{\psi} \ket{i}} = \sqrt{\bra{\psi} \sigma \ket{\psi}} = F(\ket{\psi}, \sigma)
\end{align}

Now, consider the trace distance between the probability distributions $p_m$ and $q_m$:
\begin{equation}\label{eq:trace-dist}
    D(p_m, q_m) = \frac{1}{2} \sum_{m} |p_m - q_m|
\end{equation}

This measure is upper bounded by the trace distance between the pure state $\ket{\psi}$ and the mixed state $\rho$:
\begin{equation}
    D(p_m, q_m) \leq D(\ket{\psi}, \sigma)
\end{equation}


We can prove the following:
\begin{equation}
    1 - F(\ket{\psi}, \sigma)^2 = D(p_m, q_m) \leq D(\ket{\psi}, \sigma)
\end{equation}

In particular, we can start from the trace distance between $p_m$ and $q_m$ \hyperref[eq:trace-dist]{eq:45}
\begin{align}
    D(p_m, q_m) &= \frac{1}{2} \sum_{m} |p_m - q_m| = \\
    &= \frac{1}{2} \sum_{m=0}^{r} |\bra{\psi}E_m\ket{\psi} - Tr(\sigma E_m)|
\end{align}

We have one term where $E_m = \ket{\psi}\bra{\psi}$ and $\bra{\psi}E_m\ket{\psi} = 1$, whereas we don't know the other terms.
\begin{align}
    D(p_m, q_m) &= \frac{1}{2} \left(|\bra{\psi}\ket{\psi}\bra{\psi}\ket{\psi} - \bra{\psi} \sigma \ket{\psi} | + \sum_{m=1}^{r} Tr(\sigma E_m)|\right) = \\
    &= \frac{1}{2} \left(|1 - F(\ket{\psi}, \sigma)^2 | + | \sum_{m=1}^{r} E_m Tr(\sigma)|\right)
\end{align}

Where 
\begin{equation}
    \sum_{m=0}^{r} Tr(\sigma E_m) = \bra{\psi} \sigma \ket{\psi} + \sum_{m=1}^{r} Tr(\sigma E_m) = 1
\end{equation}

Thus
\begin{equation}
    \sum_{m=1}^{r} Tr(\sigma E_m) = 1 - \bra{\psi} \sigma \ket{\psi} = 1 - F(\ket{\psi}, \sigma)^2
\end{equation}

So
\begin{align}
    D(p_m, q_m) &= \frac{1}{2} \left(|1 - F(\ket{\psi}, \sigma)^2 | + |1 - F(\ket{\psi}, \sigma)^2 |\right) = \\
    &= 1 - F(\ket{\psi}, \sigma)^2 
\end{align}

Which proves the theorem:
\begin{equation}
    1 - F(\ket{\psi}, \sigma)^2 = D(p_m, q_m) \leq D(\ket{\psi}, \sigma)
\end{equation}

\end{document}

